src/simulation/SimulationRel.v
@@ -87,11 +87,11 @@ Definition sim_res_prom (thread : thread_id) promises :=
   forall l to from (RES : Memory.get l to promises = Some (from, Message.reserve)),
   exists b b',
     ⟪ LOC  : Loc_ l b ⟫ /\
-    ⟪ RFRMWS : (<| Tid_ thread ∩₁ S \₁ I |> ;; (rfi ;; rmw)^* ;; <| Tid_ thread ∩₁ S \₁ I |>) b b' ⟫ /\
+    ⟪ RFRMWS : (⦗ Tid_ thread ∩₁ S \₁ I ⦘ ⨾ (rfi ⨾ rmw)＊ ⨾ ⦗ Tid_ thread ∩₁ S \₁ I ⦘) b b' ⟫ /\
     ⟪ FROM    : f_from b = from ⟫ /\
     ⟪ TO      : f_to b' = to ⟫ /\
-    ⟪ NOBEF   : codom_rel (<|I|> ;; rf ;; rmw) b  ⟫ /\
-    ⟪ NOAFT   : ~ dom_rel (rfi ;; rmw ;; <|Tid_ thread ∩₁ S|>) b' ⟫.
+    ⟪ NOBEF   : codom_rel (⦗I⦘ ⨾ rf ⨾ rmw) b  ⟫ /\
+    ⟪ NOAFT   : ~ dom_rel (rfi ⨾ rmw ⨾ ⦗Tid_ thread ∩₁ S⦘) b' ⟫.
 
 Definition sim_mem (thread : thread_id) (local : Local.t) mem :=
     forall l b (EB: E b) (ISSB: I b) (LOC: Loc_ l b)
@@ -142,11 +142,11 @@ Definition half_message_to_events (memory : Memory.t) :=
          (MSG : Memory.get l to memory = Some (from, Message.reserve)),
   exists b b',
     ⟪ LOC  : Loc_ l b ⟫ /\
-    ⟪ RFRMWS : (<| S \₁ I |> ;; (rf ;; rmw)^* ;; <| S \₁ I |>) b b' ⟫ /\
+    ⟪ RFRMWS : (⦗ S \₁ I ⦘ ⨾ (rf ⨾ rmw)＊ ⨾ ⦗ S \₁ I ⦘) b b' ⟫ /\
     ⟪ FROM    : f_from b = from ⟫ /\
     ⟪ TO      : f_to b' = to ⟫ /\
-    ⟪ NOBEF   : codom_rel (<|I|> ;; rf ;; rmw) b  ⟫ /\
-    ⟪ NOAFT   : ~ dom_rel (rf ;; rmw ;; <|S|>) b' ⟫.
+    ⟪ NOBEF   : codom_rel (⦗I⦘ ⨾ rf ⨾ rmw) b  ⟫ /\
+    ⟪ NOAFT   : ~ dom_rel (rf ⨾ rmw ⨾ ⦗S⦘) b' ⟫.
 
 Definition reserved_time smode memory :=
   match smode with
